WIP

Phi_Semantics_Framework/Phi_Semantics_Framework.thy
@@ -164,10 +164,17 @@ consts EqCompare :: \<open>VAL \<Rightarrow> VAL \<Rightarrow> bool\<close>
 debt_axiomatization Zero :: \<open>TY \<Rightarrow> VAL option\<close>
   where zero_well_typ: "pred_option (\<lambda>v. v \<in> Well_Type T) (Zero T)"
 
+definition has_Zero :: \<open>TY \<Rightarrow> bool\<close>
+  where \<open>has_Zero T \<longleftrightarrow> Zero T \<noteq> None\<close>
+
 lemma Zero_\<p>\<o>\<i>\<s>\<o>\<n>[simp]:
   \<open> Zero \<p>\<o>\<i>\<s>\<o>\<n> = None \<close>
   by (metis Well_Type_poison empty_iff not_None_eq option.pred_inject(2) zero_well_typ)
-  
+
+lemma has_Zero_\<p>\<o>\<i>\<s>\<o>\<n>[simp]:
+  \<open> \<not> has_Zero \<p>\<o>\<i>\<s>\<o>\<n> \<close>
+  unfolding has_Zero_def
+  by simp
 
 lemma Well_Type_unique:
   \<open>v \<in> Well_Type ta \<Longrightarrow> v \<in> Well_Type tb \<Longrightarrow> ta = tb\<close>
