Phi_Semantics/PhSm_MoV_FM.thy
@@ -6,60 +6,72 @@ section \<open>Semantics\<close>
 
 debt_axiomatization
       Map_of_Val_fm: \<open>Map_of_Val (\<m>\<a>\<p>_rep vs) =
-            (\<lambda>path. case path
-                      of AgIdx_V k # path' \<Rightarrow>
-                          (case fmlookup vs k of Some v \<Rightarrow> Map_of_Val v path'
-                                               | None \<Rightarrow> 1)
-                       | _ \<Rightarrow> 1)\<close>
+            case_list 1 (\<lambda>k'. case k'
+                  of AgIdx_V k \<Rightarrow> Map_of_Val (vs k)
+                   | _ \<Rightarrow> 1)\<close>
+
 
 \<phi>type_def ValIdx :: \<open>(VAL,'x) \<phi> \<Rightarrow> (aggregate_index, 'x) \<phi>\<close>
-  where \<open>ValIdx T \<equiv> AgIdx_V \<Zcomp>\<^sub>f T\<close>
+  where \<open>ValIdx T \<equiv> AgIdx_V o inv sVAL_emb \<Zcomp>\<^sub>f T\<close>
   deriving Basic
        and Abstract_Domain\<^sub>L
        and Functionality
        and Transformation_Functor
        and Functional_Transformation_Functor
 
-(*
+
+
+
 
 abbreviation BC_Map :: \<open>(VAL,'a) \<phi> \<Rightarrow> 'a set \<Rightarrow> (aggregate_path \<Rightarrow> 'c, 'b) \<phi> \<Rightarrow> (aggregate_path \<Rightarrow> 'c::one, 'a \<Rightarrow> 'b) \<phi> \<close>
                        ("_ \<equiv>[_]\<Rrightarrow> _" [76,20,75] 75)
   where \<open>BC_Map K D V \<equiv> \<phi>MapTree D (ValIdx K) V\<close>
 
-term \<open> (f \<Ztypecolon> \<m>\<e>\<m>-\<c>\<o>\<e>\<r>\<c>\<e> MapVal D K V) \<close>
+term \<open> (f \<Ztypecolon> \<m>\<e>\<m>-\<c>\<o>\<e>\<r>\<c>\<e> MapVal K V) \<close>
 term \<open> (f \<Ztypecolon> K \<equiv>[D]\<Rrightarrow> \<m>\<e>\<m>-\<c>\<o>\<e>\<r>\<c>\<e> V) \<close>
-*)
+
 
 
 setup \<open>Context.theory_map ( Phi_Mem_Printer.add 110 (
-    fn (ctxt, f, Const(\<^const_syntax>\<open>Phi_Types.\<phi>MapTree\<close>, _)
-          $ D
-          $ (Const(\<^const_syntax>\<open>ValIdx\<close>, _) $ K)
-          $ V) =>
-        SOME (Const(\<^const_syntax>\<open>MapVal\<close>, dummyT) $ D $ K $ f ctxt V)
+    fn (ctxt, f, Const(\<^const_syntax>\<open>BC_Map\<close>, _) $ D $ K $ V) =>
+        SOME (Const(\<^const_syntax>\<open>BC_Map\<close>, dummyT) $ D $ K $ f ctxt V)
      | _ => NONE
   )
 )\<close>
 
 setup \<open>Context.theory_map ( Phi_Mem_Parser.add 110 (
-    fn (ctxt, f, Const(\<^const_syntax>\<open>MapVal\<close>, _) $ D $ K $ V) =>
-        SOME (Const(\<^const_syntax>\<open>\<phi>MapTree\<close>, dummyT)
-                $ D $ (Const(\<^const_syntax>\<open>ValIdx\<close>, dummyT) $ K) $ f ctxt V)
+    fn (ctxt, f, Const(\<^const_syntax>\<open>BC_Map\<close>, _) $ D $ K $ V) =>
+        SOME (Const(\<^const_syntax>\<open>BC_Map\<close>, dummyT) $ D $ K $ f ctxt V)
      | X => NONE
   )
 )\<close>
 
-term \<open>\<m>\<e>\<m>-\<c>\<o>\<e>\<r>\<c>\<e> MapVal D K V\<close>
+
+
+term \<open>A \<equiv>\<Rrightarrow> B\<close>
+
+term \<open>\<m>\<e>\<m>-\<c>\<o>\<e>\<r>\<c>\<e> MapVal K V\<close>
 term \<open>\<phi>MapTree D (ValIdx K) (\<m>\<e>\<m>-\<c>\<o>\<e>\<r>\<c>\<e> V)\<close>
 
-term \<open>\<m>\<e>\<m>[addr] (\<m>\<e>\<m>-\<c>\<o>\<e>\<r>\<c>\<e> MapVal D K V)\<close>
+term \<open>\<m>\<e>\<m>[addr] (\<m>\<e>\<m>-\<c>\<o>\<e>\<r>\<c>\<e> MapVal K V)\<close>
 term \<open>\<m>\<e>\<m>[addr] (\<phi>MapTree D (ValIdx K) (\<m>\<e>\<m>-\<c>\<o>\<e>\<r>\<c>\<e> V))\<close>
 term \<open>\<m>\<e>\<m>[addr] (K \<equiv>[D]\<Rrightarrow> (V::(VAL,'x)\<phi>))\<close>
 
-term \<open>\<m>\<e>\<m>[addr] MapVal D K V\<close>
-ML \<open>@{term \<open>\<m>\<e>\<m>[addr] MapVal D K V\<close>}\<close>
+term \<open>\<m>\<e>\<m>[addr] MapVal K V\<close>
+ML \<open>@{term \<open>\<m>\<e>\<m>[addr] MapVal K V\<close>}\<close>
 
+text \<open>Intuitively, \<open>\<phi>VM_Domain D K V\<close> specifies the domain\<close>
 
+definition \<phi>VM_Domain :: \<open>(VAL,'x) \<phi> \<Rightarrow> TY \<Rightarrow> mem_fic BI\<close>
+     where \<open>\<phi>VM_Domain K V \<equiv> case_list 1 (\<lambda>k'.
+                case k' of AgIdx_V k \<Rightarrow>
+                      (if (\<exists>k. k' = concretize (ValIdx K) k) then 1
+                       else (to_share o map_option discrete o Map_of_Val (the (Zero V))))
+                   | _ \<Rightarrow> 1) \<Ztypecolon> Itself \<close>
+
+setup \<open>Sign.mandatory_path "\<phi>VM_Domain"\<close>
+
+setup \<open>Sign.parent_path\<close>
 
 
 lemma pull_map_map_option:
@@ -71,18 +83,22 @@ lemma map_option_o_eq_inj:
   \<open> inj f
 \<Longrightarrow> map_option f o g = map_option f o g' \<longleftrightarrow> g = g'\<close>
   by (meson fun.inj_map injD option.inj_map)
-  
+
+(*
 lemma pull_map__Map_of_Val_\<m>\<a>\<p>__in_dom:
   \<open> k \<in> fmdom' f
-\<Longrightarrow> pull_map [AgIdx_V k] (Map_of_Val (\<m>\<a>\<p>_rep f)) = Map_of_Val (the (fmlookup f k))\<close>
+\<Longrightarrow> pull_map [AgIdx_V k] (Map_of_Val (\<m>\<a>\<p>_rep (f,U))) = Map_of_Val (the (fmlookup f k))\<close>
   unfolding Map_of_Val_fm fun_eq_iff pull_map_def
   by (auto, meson fmdom'_notI option.case_eq_if)
+*)
+
+
 
 
 lemma Map_of_Val_\<m>\<a>\<p>_Nil:
   \<open> Map_of_Val (\<m>\<a>\<p>_rep xa) [] = 1 \<close>
-  unfolding Map_of_Val_fm fun_eq_iff
-  by auto
+  unfolding fun_eq_iff
+  by (auto simp: Map_of_Val_fm)
 
 lemma to_share_inj [simp]:
   \<open>to_share x = to_share y \<longleftrightarrow> x = y\<close>
@@ -93,49 +109,116 @@ lemma map_option_inj:
 \<Longrightarrow> map_option f x = map_option f y \<longleftrightarrow> x = y \<close>
   by (meson injD option.inj_map)
 
-lemma mem_coerce_MapVal:
-  \<open> Abstract_Domain\<^sub>L K (\<lambda>x. x \<in> D)
-\<Longrightarrow> Functionality K (\<lambda>x. x \<in> D)
-\<Longrightarrow> Injective_on K D
-\<Longrightarrow> finite D
-\<Longrightarrow> \<m>\<e>\<m>-\<c>\<o>\<e>\<r>\<c>\<e> MapVal D K V = \<phi>MapTree D (ValIdx K) (\<m>\<e>\<m>-\<c>\<o>\<e>\<r>\<c>\<e> V) \<close>
+term \<open>{c. \<exists>x. c \<Turnstile> (x \<Ztypecolon> T) \<and> x \<in> D } = Well_Type TY\<^sub>K \<close>
 
-  apply (rule \<phi>Type_eqI, clarify)
-  subgoal premises prems for f u proof -
-    have t1: \<open> k \<in> D \<Longrightarrow> concretize (ValIdx K) k = AgIdx_V (concretize K k) \<close> for k
-      by (smt (verit, best) Abstract_Domain\<^sub>L_def Functionality_def ValIdx.Abstract_Domain\<^sub>L ValIdx.expansion \<r>ESC_def concretize_SAT prems)
+
+lemma pull_map__case_list[simp]:
+  \<open> pull_map [k] (case_list x F) = F k \<close>
+  unfolding pull_map_def
+  by simp
+
+
+
+lemma mem_coerce_MapVal:
+  \<open> Abstract_Domain\<^sub>L K (\<lambda>x. True)
+\<Longrightarrow> Functionality K (\<lambda>x. True)
+\<Longrightarrow> Injective_on K UNIV
+\<Longrightarrow> Semantic_Type K TY\<^sub>K
+\<Longrightarrow> \<c>\<o>\<n>\<d>\<i>\<t>\<i>\<o>\<n> \<t>\<y>\<p>\<e>\<o>\<f> V = TY\<^sub>V \<and> TY\<^sub>V \<noteq> \<p>\<o>\<i>\<s>\<o>\<n> \<and> is_sTY TY\<^sub>K
+\<Longrightarrow> f \<Ztypecolon> \<m>\<e>\<m>-\<c>\<o>\<e>\<r>\<c>\<e> MapVal K V \<equiv> (f \<Ztypecolon> \<phi>MapTree UNIV (ValIdx K) (\<m>\<e>\<m>-\<c>\<o>\<e>\<r>\<c>\<e> V)) * \<phi>VM_Domain K TY\<^sub>V \<close>
+  unfolding atomize_eq BI_eq_iff Semantic_Zero_Val_def Premise_def
+  apply (clarify)
+  subgoal premises prems for u proof -
+
+    have t01: \<open>inj (concretize K)\<close>
+      by (simp add: concretize_inj prems(1) prems(3))
+
+    have t02[simp]: \<open>concretize K a = concretize K b \<longleftrightarrow> a = b\<close> for a b
+      by (meson injD t01)
+
+    have t03: \<open>v = concretize K x \<longleftrightarrow> v \<Turnstile> (x \<Ztypecolon> K)\<close> for x v
+      by (metis Abstract_Domain\<^sub>L_def Functionality_def \<r>ESC_def concretize_SAT prems(1) prems(2))
+
+    have [simp]: \<open>\<t>\<y>\<p>\<e>\<o>\<f> V = TY\<^sub>V\<close> using prems(5) by fastforce
+
+    have t1: \<open> concretize (ValIdx K) k = AgIdx_V (inv sVAL_emb (concretize K k)) \<close> for k
+      by (metis Abstract_Domain\<^sub>L_def ValIdx.Abstract_Domain\<^sub>L ValIdx.expansion \<r>ESC_def comp_apply concretize_SAT prems(1) t03)
+
+    let ?M1 = \<open>\<lambda>g k. if (\<exists>kk. sVAL_emb k = concretize K kk) then Map_of_Val (g k) else 1\<close>
+    let ?M2 = \<open>\<lambda>g k. if (\<exists>kk. sVAL_emb k = concretize K kk) then 1 else Map_of_Val (g k)\<close>
+
+    have Map_of_Val__\<m>\<a>\<p>_rep__split:
+      \<open> Map_of_Val (\<m>\<a>\<p>_rep g) =
+          case_list 1 (\<lambda>k'. case k' of AgIdx_V k \<Rightarrow> ?M1 g k | _ \<Rightarrow> 1) *
+          case_list 1 (\<lambda>k'. case k' of AgIdx_V k \<Rightarrow> ?M2 g k | _ \<Rightarrow> 1) \<close>
+      for g
+      unfolding Map_of_Val_fm fun_eq_iff
+      by (clarify, case_tac x, auto split: option.split aggregate_index'.split
+                                    simp: fun_eq_iff fmdom'_notI times_fun)
+
+    have t2: \<open>
+      to_share \<circ> (map_option discrete \<circ> Map_of_Val (\<m>\<a>\<p>_rep g)) =
+        (to_share \<circ> (map_option discrete \<circ> case_list 1 (\<lambda>k'. case k' of AgIdx_V k \<Rightarrow> ?M1 g k | _ \<Rightarrow> 1))) *
+        (to_share \<circ> (map_option discrete \<circ> case_list 1 (\<lambda>k'. case k' of AgIdx_V k \<Rightarrow> ?M2 g k | _ \<Rightarrow> 1)))\<close>
+      for g
+    unfolding Map_of_Val__\<m>\<a>\<p>_rep__split fun_eq_iff
+    by (clarify; case_tac x; auto split: aggregate_index'.split option.split simp: times_fun prems(4))
+
+    have t3[simp]: \<open>sVAL_emb (inv sVAL_emb (concretize K k)) = concretize K k\<close> for k
+      by (meson Semantic_Type_def f_inv_into_f is_sTY prems(4) prems(7) t03)
+
+
     show ?thesis
     apply (auto simp: pull_map_to_share comp_assoc pull_map_map_option map_option_o_eq_inj
-                      pull_map__Map_of_Val_\<m>\<a>\<p>__in_dom t1 Map_of_Val_\<m>\<a>\<p>_Nil)
-    apply (clarsimp simp add: Map_of_Val_fm split: aggregate_index'.split option.split)
-     apply (metis fmdom'I imageE)
-    subgoal premises prems2 proof -
-      obtain v where t2: \<open>k \<in> D \<Longrightarrow> pull_map [AgIdx_V (concretize K k)] u = to_share \<circ> (map_option discrete \<circ> Map_of_Val (v k)) \<and> v k \<Turnstile> (f k \<Ztypecolon> V)\<close> for k
-        using prems2(1) by metis
-      let ?g = \<open>\<lambda>k. if (\<exists>k'\<in>D. k = concretize K k') then Some (v (inv_into D (concretize K) k)) else None\<close>
+                      t1 Map_of_Val_\<m>\<a>\<p>_Nil)
+subgoal for g
+apply (rule exI[where x=\<open>to_share \<circ> (map_option discrete \<circ> (case_list 1 (\<lambda>k'.
+                      case k' of AgIdx_V k \<Rightarrow> ?M1 g k | _ \<Rightarrow> 1 )))\<close>])
+apply (rule exI[where x=\<open>to_share \<circ> (map_option discrete \<circ> (case_list 1 (\<lambda>k'.
+                      case k' of AgIdx_V k \<Rightarrow> ?M2 g k | _ \<Rightarrow> 1 )))\<close>])
+ apply (auto simp: pull_map_to_share comp_assoc pull_map_map_option map_option_o_eq_inj
+                   t2 t1 Map_of_Val_\<m>\<a>\<p>_Nil sep_disj_fun_def
+             split: option.split aggregate_index'.split list.split)
+  using t03 t3 apply blast
+  apply (metis inj_sVAL_emb inv_f_f)
+
+apply (insert t03, auto simp: \<phi>VM_Domain_def fun_eq_iff t1 inj_sVAL_emb inv_f_f split: option.split list.split aggregate_index'.split)
+  apply (metis inj_sVAL_emb inv_f_f)
+  apply blast .
   
-      have t3: \<open>{a. \<exists>k'\<in>D. a = concretize K k'} \<subseteq> concretize K ` D\<close>
+
+
+apply (auto simp add: \<phi>VM_Domain_def)
+subgoal premises prems2 for u'
+
+ proof -
+thm prems2
+      obtain v where t2: \<open>pull_map [AgIdx_V (inv sVAL_emb (concretize K k))] u' = to_share \<circ> (map_option discrete \<circ> Map_of_Val (v k)) \<and> v k \<Turnstile> (f k \<Ztypecolon> V)\<close> for k
+        using prems2(2) by metis
+      let ?g = \<open>\<lambda>k. if (\<exists>k'. k = concretize K k') then v (inv (concretize K) k) else the (Zero TY\<^sub>V)\<close>
+  
+      have t3: \<open>{a. \<exists>k'. a = concretize K k'} \<subseteq> concretize K ` UNIV\<close>
         unfolding set_eq_iff
         by (auto simp: image_iff Bex_def)
-  
-      have t4[simp]: \<open>fmlookup (Abs_fmap ?g) = ?g\<close>
-        by (rule fmap.Abs_fmap_inverse, auto simp: dom_def prems(4))
-  
-      have t5: \<open>k \<in> D \<Longrightarrow> inv_into D (concretize K) (concretize K k) = k\<close> for k
+    
+      have t5: \<open>inv (concretize K) (concretize K k) = k\<close> for k
         by (simp add: concretize_inj prems(1) prems(3))
   
       show ?thesis
-        apply (rule exI[where x=\<open>\<m>\<a>\<p>_rep (Abs_fmap ?g)\<close>])
-        apply (auto simp: fun_eq_iff Map_of_Val_fm split: list.split aggregate_index'.split)
-        apply (simp add: prems2(2))
-        using prems2(3) apply blast
-        using prems2(3) apply blast
-        subgoal premises prem3 for x22 k'
-          by (insert t2[OF prem3], auto simp: pull_map_def fun_eq_iff map_option_inj t5 prem3)
-        apply (simp add: prems2(3))
-        apply (metis (no_types, lifting) fmdom'_notI image_iff t4)
-        apply (metis (no_types, lifting) domIff fmdom'.rep_eq option.distinct(1) t4)
-        by (metis t2 t5)
+        apply (rule exI[where x=\<open>\<m>\<a>\<p>_rep (?g o sVAL_emb)\<close>])
+        apply (auto simp: fun_eq_iff Map_of_Val_fm prems2(3,4) t1 t5 times_fun
+                    split: list.split aggregate_index'.split)
+        apply (metis append.simps(1) append.simps(2) comp_apply pull_map_def t2)
+        apply (metis inj_sVAL_emb inv_f_f)
+
+        apply (rule exI[where x=\<open>\<lambda>xa. if (\<exists>k'. sVAL_emb xa = concretize K k') then v (inv (concretize K) (sVAL_emb xa)) else the (Zero TY\<^sub>V)\<close>],
+               auto)
+        apply (metis Inhabited_def SType_Of_def Semantic_Type_def Well_Type_unique concretize_SAT is_sTY_poison prems(4) prems(7) someI_ex)
+        apply (metis Abstract_Domain\<^sub>L_def Inhabited_def SType_Of_not_poison Semantic_Type_def \<r>ESC_def prems(1) prems(4))
+        using prems(6) apply fastforce
+        apply (metis t03 t2 t5)
+        using t03 apply blast
+        using t03 by blast
     qed .
   qed .
 
@@ -150,7 +233,6 @@ lemma [\<phi>reason %mapToA_mem_coerce,
   \<open> Abstract_Domain\<^sub>L K (\<lambda>x. x \<in> D)
 \<Longrightarrow> Functionality K (\<lambda>x. x \<in> D)
 \<Longrightarrow> Injective_on K D
-\<Longrightarrow> finite D
 
 \<Longrightarrow> \<m>\<a>\<p> g : \<phi>MapTree D (ValIdx K) (\<m>\<e>\<m>-\<c>\<o>\<e>\<r>\<c>\<e>[TYU] V) \<OTast> R
          \<mapsto> \<phi>MapTree D (ValIdx K) (\<m>\<e>\<m>-\<c>\<o>\<e>\<r>\<c>\<e> V') \<OTast> R'
@@ -171,24 +253,67 @@ lemma [\<phi>reason %mapToA_mem_coerce,
   \<open> Abstract_Domain\<^sub>L K (\<lambda>x. x \<in> D)
 \<Longrightarrow> Functionality K (\<lambda>x. x \<in> D)
 \<Longrightarrow> Injective_on K D
-\<Longrightarrow> finite D
 
 \<Longrightarrow> \<m>\<a>\<p> g : U \<OTast> R \<mapsto> U' \<OTast> R'
-    \<o>\<v>\<e>\<r> f : \<phi>MapTree D (ValIdx K) (\<m>\<e>\<m>-\<c>\<o>\<e>\<r>\<c>\<e>[TYU] V) \<OTast> W
+    \<o>\<v>\<e>\<r> f : \<phi>MapTree D (ValIdx K) (\<m>\<e>\<m>-\<c>\<o>\<e>\<r>\<c>\<e>[TYV] V) \<OTast> W
           \<mapsto> \<phi>MapTree D (ValIdx K) (\<m>\<e>\<m>-\<c>\<o>\<e>\<r>\<c>\<e> V') \<OTast> W'
     \<w>\<i>\<t>\<h> \<g>\<e>\<t>\<t>\<e>\<r> getter \<s>\<e>\<t>\<t>\<e>\<r> setter \<i>\<n> DD
 
 \<Longrightarrow> \<m>\<a>\<p> g : U \<OTast> R \<mapsto> U' \<OTast> R'
-    \<o>\<v>\<e>\<r> f : \<m>\<e>\<m>-\<c>\<o>\<e>\<r>\<c>\<e>[\<m>\<a>\<p>[TYK,TYU]] (MapVal D K V) \<OTast> W
+    \<o>\<v>\<e>\<r> f : \<m>\<e>\<m>-\<c>\<o>\<e>\<r>\<c>\<e>[\<m>\<a>\<p>[TYK,TYV]] (MapVal D K V) \<OTast> W
           \<mapsto> \<m>\<e>\<m>-\<c>\<o>\<e>\<r>\<c>\<e> (MapVal D K V') \<OTast> W'
     \<w>\<i>\<t>\<h> \<g>\<e>\<t>\<t>\<e>\<r> getter \<s>\<e>\<t>\<t>\<e>\<r> setter \<i>\<n> DD \<close>
 
   unfolding Guided_Mem_Coercion_def mem_coerce_MapVal .
 
 
+subsubsection \<open>Transformation\<close>
 
+lemma [\<phi>reason %ToA_mem_coerce,
+       unfolded Guided_Mem_Coercion_def,
+       \<phi>reason %ToA_mem_coerce]:
 
+  \<open> Abstract_Domain\<^sub>L K (\<lambda>x. x \<in> D)
+\<Longrightarrow> Functionality K (\<lambda>x. x \<in> D)
+\<Longrightarrow> Injective_on K D
 
+\<Longrightarrow> x \<Ztypecolon> \<phi>MapTree D (ValIdx K) (\<m>\<e>\<m>-\<c>\<o>\<e>\<r>\<c>\<e>[TYV] V') \<t>\<r>\<a>\<n>\<s>\<f>\<o>\<r>\<m>\<s> Y \<w>\<i>\<t>\<h> P
+\<Longrightarrow> x \<Ztypecolon> \<m>\<e>\<m>-\<c>\<o>\<e>\<r>\<c>\<e>[\<m>\<a>\<p>[TYK,TYU]] (MapVal D K V') \<t>\<r>\<a>\<n>\<s>\<f>\<o>\<r>\<m>\<s> Y \<w>\<i>\<t>\<h> P \<close>
+
+  unfolding Guided_Mem_Coercion_def mem_coerce_MapVal .
+
+lemma [\<phi>reason %ToA_mem_coerce,
+       unfolded Guided_Mem_Coercion_def,
+       \<phi>reason %ToA_mem_coerce]:
+  \<open> Abstract_Domain\<^sub>L K (\<lambda>x. x \<in> D)
+\<Longrightarrow> Functionality K (\<lambda>x. x \<in> D)
+\<Longrightarrow> Injective_on K D
+
+\<Longrightarrow> x \<Ztypecolon> \<phi>MapTree D (ValIdx K) (\<m>\<e>\<m>-\<c>\<o>\<e>\<r>\<c>\<e>[TYV] V) \<OTast> W \<t>\<r>\<a>\<n>\<s>\<f>\<o>\<r>\<m>\<s> Y \<w>\<i>\<t>\<h> P
+\<Longrightarrow> x \<Ztypecolon> \<m>\<e>\<m>-\<c>\<o>\<e>\<r>\<c>\<e>[\<m>\<a>\<p>[TYK,TYU]] (MapVal D K V) \<OTast> W \<t>\<r>\<a>\<n>\<s>\<f>\<o>\<r>\<m>\<s> Y \<w>\<i>\<t>\<h> P \<close>
+  unfolding Guided_Mem_Coercion_def mem_coerce_MapVal .
+
+lemma [\<phi>reason %ToA_mem_coerce,
+       unfolded Guided_Mem_Coercion_def,
+       \<phi>reason %ToA_mem_coerce]:
+  \<open> Abstract_Domain\<^sub>L K (\<lambda>x. x \<in> D)
+\<Longrightarrow> Functionality K (\<lambda>x. x \<in> D)
+\<Longrightarrow> Injective_on K D
+
+\<Longrightarrow> X \<t>\<r>\<a>\<n>\<s>\<f>\<o>\<r>\<m>\<s> x \<Ztypecolon> \<phi>MapTree D (ValIdx K) (\<m>\<e>\<m>-\<c>\<o>\<e>\<r>\<c>\<e>[TYV] V) \<w>\<i>\<t>\<h> P
+\<Longrightarrow> X \<t>\<r>\<a>\<n>\<s>\<f>\<o>\<r>\<m>\<s> x \<Ztypecolon> \<m>\<e>\<m>-\<c>\<o>\<e>\<r>\<c>\<e>[\<m>\<a>\<p>[TYK,TYU]] (MapVal D K V) \<w>\<i>\<t>\<h> P \<close>
+  unfolding Guided_Mem_Coercion_def mem_coerce_MapVal .
+
+lemma [\<phi>reason %ToA_mem_coerce,
+       unfolded Guided_Mem_Coercion_def,
+       \<phi>reason %ToA_mem_coerce]:
+  \<open> Abstract_Domain\<^sub>L K (\<lambda>x. x \<in> D)
+\<Longrightarrow> Functionality K (\<lambda>x. x \<in> D)
+\<Longrightarrow> Injective_on K D
+
+\<Longrightarrow> X \<t>\<r>\<a>\<n>\<s>\<f>\<o>\<r>\<m>\<s> x \<Ztypecolon> \<phi>MapTree D (ValIdx K) (\<m>\<e>\<m>-\<c>\<o>\<e>\<r>\<c>\<e>[TYV] V) \<OTast> R \<w>\<i>\<t>\<h> P
+\<Longrightarrow> X \<t>\<r>\<a>\<n>\<s>\<f>\<o>\<r>\<m>\<s> x \<Ztypecolon> \<m>\<e>\<m>-\<c>\<o>\<e>\<r>\<c>\<e>[\<m>\<a>\<p>[TYK,TYU]] (MapVal D K V) \<OTast> R \<w>\<i>\<t>\<h> P \<close>
+  unfolding Guided_Mem_Coercion_def mem_coerce_MapVal .
 
 
 
